src/cbor/pulse/raw/CBOR.Pulse.Raw.Format.Serialized.Iterator.fsti
@@ -1,0 +1,7 @@
+module CBOR.Pulse.Raw.Format.Serialized.Iterator
+
+[@@CAbstractStruct]
+val cbor_serialized_array_iterator: Type0
+
+[@@CAbstractStruct]
+val cbor_serialized_map_iterator: Type0
